sketch some edits with @wildptr

compiler/backend/proofs/word_copyProofScript.sml
@@ -10,15 +10,23 @@ val s = ``s:('a,'c,'ffi) wordSem$state``
 val _ = set_grammar_ancestry ["wordLang", "wordSem", "wordProps", "word_copy"];
 
 Definition CPstate_inv_def:
-  CPstate_inv cs =
-  ((∀v c. lookup v cs.to_eq = SOME c ⇒ c < cs.next) ∧
+  CPstate_inv cs = (
+   (* cs.next is a fresh class *)
+   (∀v c. lookup v cs.to_eq = SOME c ⇒ c < cs.next) ∧
+   (∀c. c ∈ domain cs.from_eq ⇒ c < cs.next) ∧
    (* each class has a representative *)
-   (∀c. c < cs.next ⇒ lookup c cs.from_eq ≠ NONE) ∧
-   (* if representative of equiv class c is var v, then class of v is c *)
-   (∀c v. c < cs.next ⇒  lookup c cs.from_eq = SOME v ⇒ lookup v cs.to_eq = SOME c) ∧
+   (* (∀c. c < cs.next ⇒ lookup c cs.from_eq ≠ NONE) ∧
+   *)
+   (* if representative of equiv class c is var v,
+      then class of v is c *)
+   (∀c v. lookup c cs.from_eq = SOME v ⇒
+     lookup v cs.to_eq = SOME c)
+  )
+End
+(*   ∧
    (* different classes have different representatives *)
    (∀c c'. c < c' ⇒ c' < cs.next ⇒ lookup c cs.from_eq ≠ lookup c' cs.from_eq))
-End
+End *)
 
 Theorem empty_eq_inv:
   CPstate_inv empty_eq
@@ -27,89 +35,152 @@ Proof
 QED
 
 Theorem remove_eq_inv:
-  ∀cs v. CPstate_inv cs ⇒ CPstate_inv (remove_eq cs v)
+  ∀cs v. CPstate_inv cs ⇒
+  CPstate_inv (remove_eq cs v)
 Proof
-  rw[remove_eq_def]>>Cases_on‘lookup v cs.to_eq’>>rw[empty_eq_inv]
+  rw[remove_eq_def]>>
+  Cases_on‘lookup v cs.to_eq’>>
+  rw[empty_eq_inv]
 QED
 
 Theorem remove_eqs_inv:
-  ∀vv cs. CPstate_inv cs ⇒ CPstate_inv (remove_eqs cs vv)
+  ∀vv cs. CPstate_inv cs ⇒
+    CPstate_inv (remove_eqs cs vv)
 Proof
-  Induct_on‘vv’>>rw[remove_eqs_def,remove_eq_inv]
+  Induct>>
+  rw[remove_eqs_def,remove_eq_inv]
 QED
 
 Theorem set_eq_inv:
   ∀cs t s.
-   CPstate_inv cs ⇒
-   lookup t cs.to_eq = NONE ⇒
-   CPstate_inv (set_eq cs t s)
+    CPstate_inv cs ∧
+    lookup t cs.to_eq = NONE ⇒
+    CPstate_inv (set_eq cs t s)
 Proof
   rpt strip_tac>>
-  ‘∀c. c<cs.next ⇒ lookup c cs.from_eq ≠ SOME t’
-    by (fs[CPstate_inv_def]>>metis_tac[NOT_NONE_SOME])>>
-  Cases_on‘is_alloc_var t ∧ is_alloc_var s’THENL
-  [
-    namedCases_on‘lookup s cs.to_eq’["","c_s"]THENL
-    [
-      (* lookup s cs.to_eq = NONE *)
-      last_x_assum mp_tac>>
-      rw[CPstate_inv_def,set_eq_def]THENL
-      [
-        (* inv. 1 *)
-        qpat_x_assum‘_=SOME c’mp_tac>>
-        rewrite_tac[lookup_insert]>>
-        (Cases_on‘v=t’>-rw[])>>
-        (Cases_on‘v=s’>-rw[])>>
-        rw[]>>
-        ‘c<cs.next’ by metis_tac[]>>
-        decide_tac,
-        (* inv. 2 *)
-        rw[lookup_insert]>>
-        qpat_x_assum‘_=SOME v’mp_tac>>
-        rw[lookup_insert]>>
-        metis_tac[]>>
-        ‘c<cs.next’ by decide_tac>>
-        metis_tac[NOT_NONE_SOME],
-        (* inv. 3 *)
-        rw[lookup_insert]>-(
-          qpat_x_assum‘_=SOME t’mp_tac>>
-          rw[lookup_insert]>>
-          qpat_x_assum‘_=SOME s’mp_tac>>
-          rw[lookup_insert]>>
-          ‘c<cs.next’ by decide_tac>>
-          metis_tac[NOT_NONE_SOME]
-          )>>
-        qpat_x_assum‘_=SOME v’mp_tac>>
-        (Cases_on‘c=cs.next’>-rw[lookup_insert])>>
-        ‘c<cs.next’ by decide_tac>>rw[lookup_insert]>>
-        metis_tac[NOT_NONE_SOME],
-        (* inv. 4 *)
-        ‘c<cs.next’ by decide_tac>>
-        rw[lookup_insert]
-      ],
-      (* lookup s cs.to_eq = SOME c_s *)
-      last_x_assum mp_tac>>
-      rw[CPstate_inv_def,set_eq_def]THENL
-      [
-        (* inv. 1 *)
-        qpat_x_assum‘_=SOME c’mp_tac>>
-        rewrite_tac[lookup_insert]>>
-        Cases_on‘v=t’>>Cases_on‘v=s’>>metis_tac[NOT_NONE_SOME],
-        (* inv. 2 *)
-        Cases_on‘c=c_s’>>asm_rewrite_tac[lookup_insert]>-rw[]>>
-        metis_tac[],
-        (* inv. 3 *)
-        Cases_on‘v=t’>>asm_rewrite_tac[lookup_insert]>-metis_tac[lookup_insert,NOT_NONE_SOME]>>
-        ‘lookup c cs.from_eq = SOME v’by(
-          qpat_x_assum‘_=SOME v’mp_tac>>
-          Cases_on‘c=c_s’>>rw[lookup_insert]>>metis_tac[NOT_NONE_SOME])>>
-        rw[lookup_insert],
-        (* inv. 4 *)
-        rw[lookup_insert]
-      ]
-    ],
-    rw[set_eq_def]
-  ]
+  ‘∀c. lookup c cs.from_eq ≠ SOME t’ by (
+    fs[CPstate_inv_def]>>
+    metis_tac[NOT_NONE_SOME])>>
+  rw[set_eq_def]>>
+  namedCases_on‘lookup s cs.to_eq’["","c_s"]>>
+  fs[]
+  >~[`lookup s cs.to_eq = NONE`]
+  >- (
+    fs[CPstate_inv_def]>>
+    rw[lookup_insert]>>simp[]
+    >- (
+      first_x_assum drule>>
+      simp[])
+    >- (
+      first_x_assum drule>>
+      simp[])
+    >- metis_tac[NOT_SOME_NONE])
+  >~[`lookup s cs.to_eq = SOME c_s`]
+  >- (
+    fs[CPstate_inv_def]>>
+    rw[lookup_insert]>>
+    metis_tac[])
+QED
+
+(*
+Theorem set_eq_inv:
+  ∀cs t s.
+    CPstate_inv cs ∧
+    lookup t cs.to_eq = NONE ⇒
+    CPstate_inv (set_eq cs t s)
+Proof
+  rpt strip_tac>>
+  ‘∀c. c<cs.next ⇒ lookup c cs.from_eq ≠ SOME t’ by (
+    fs[CPstate_inv_def]>>
+    metis_tac[NOT_NONE_SOME])>>
+  rw[set_eq_def]>>
+  namedCases_on‘lookup s cs.to_eq’["","c_s"]>>
+  fs[]
+  >~[`lookup s cs.to_eq = NONE`]
+  >- (
+    fs[CPstate_inv_def]>>
+    rw[lookup_insert]
+    >- (
+      first_x_assum drule>>
+      simp[])>>
+    ‘c<cs.next’ by decide_tac>>
+    metis_tac[NOT_NONE_SOME])
+  >~[`lookup s cs.to_eq = SOME c_s`]
+  >- (
+    fs[CPstate_inv_def]>>
+    rw[lookup_insert]>>
+    metis_tac[])
+QED
+*)
+
+Theorem merge_eqs_inv:
+  CPstate_inv cs ∧
+  CPstate_inv ds ⇒
+  CPstate_inv (merge_eqs cs ds)
+Proof
+  rw[]>>
+  simp[merge_eqs_def,CPstate_inv_def]>>
+  CONJ_TAC >- (
+    (* invariant 1 works *)
+    rw[lookup_inter_eq]>>gvs[AllCaseEqs()]>>
+    metis_tac[CPstate_inv_def] ) >>
+  CONJ_TAC >- (
+    (* invariant 2 works *)
+    simp[domain_lookup,lookup_inter_eq,AllCaseEqs()]>>
+    rw[]>>
+    cheat )>>
+  rw[lookup_inter_eq,AllCaseEqs()]>>
+  metis_tac[CPstate_inv_def]
+QED
+
+Theorem same_classD:
+  CPstate_inv cs ∧
+  lookup_eq cs x = lookup_eq cs y ⇒
+  x = y ∨
+  (∃c.
+    lookup x cs.to_eq = SOME c ∧
+    lookup y cs.to_eq = SOME c)
+Proof
+  rw[lookup_eq_def,AllCaseEqs()]
+  >- (
+    fs[CPstate_inv_def]>>
+    metis_tac[NOT_NONE_SOME])
+  >- (
+    fs[CPstate_inv_def]>>
+    first_x_assum drule>>
+    rw[])>>
+  Cases_on`lookup y cs.to_eq`>>gvs[]
+  >- (
+    fs[CPstate_inv_def]>>
+    metis_tac[NOT_NONE_SOME])>>
+  rename1`lookup y _ = SOME cy`>>
+  Cases_on`lookup cy cs.from_eq`>>gvs[]
+  >- (
+    fs[CPstate_inv_def]>>
+    first_x_assum drule>>
+    rw[])>>
+  fs[CPstate_inv_def]>>
+  metis_tac[SOME_11]
+QED
+
+Theorem lookup_eq_set_eq_not_is_alloc_var:
+  ¬ (is_alloc_var s ∧ is_alloc_var t) ⇒
+  lookup_eq (set_eq cs t s) v =
+  lookup_eq cs v
+Proof
+  rw[set_eq_def]
+QED
+
+(* t := s *)
+Theorem lookup_eq_set_eq_is_alloc_var:
+  CPstate_inv cs ∧
+  is_alloc_var s ∧ is_alloc_var t ⇒
+  lookup_eq (set_eq cs t s) v =
+  if lookup_eq cs s = lookup_eq cs v
+  then t
+  else lookup_eq cs v
+Proof
+  cheat
 QED
 
 (* TODO: insert an induction over copy_prop_prog *)
